\begin{frame}
  \frametitle{Layered Approach}

  Since \Uf is the empty theory, it is contained in any other theory \T. So the following
  implication holds
  \begin{center}
  If a conjunction $\varphi$ is \Uf-unsatisfiable, then it is \T-unsatisfiable
  \end{center}
  \vfill
  Example:
  $$
    x + y \not= z + w\quad\wedge\quad x = z\quad\wedge\quad y = w
  $$
  is an \Lra-formula, but it is \Uf-unsatisfiable\pause
  $$
    plus(x,y) \not= plus(z,w)\quad\wedge\quad x = z\quad\wedge\quad y = w
  $$
  \vfill\pause
  Therefore we can use \Uf-solver as a layer for \Lra-solver on an input conjunction $\varphi$:
  \begin{itemize}
    \item Call \Uf-solver on $\varphi$. If $unsat$ return $unsat$
    \item Call \Lra-solver on $\varphi$
  \end{itemize}
  This can save many calls to \Lra-solver. Since \Uf-solver is quick, this can save time !

\end{frame}

\begin{frame}[fragile]
  \frametitle{Exercises}

  \begin{enumerate}
    \item Prove by induction the invariant on slide 9
    \vfill
    \item Write the precise pseudocode for Explain
    \vfill
    \item Is the following conjunction satisfiable ?
          $$
	    f(g(x))\!\not=\!f(y)\ \wedge\ x\!=\!w\ \wedge\ g(x)\!=\!h(z)\ \wedge\ z\!=\!x\ \wedge\ h(w)\!=\!y  
	  $$
    \vfill
    \item Verify your anwser using an SMT-solver of your choice. In smtlib2 the above
          can be written as
	  \begin{verbatim}
          (set-logic QF_UF)
          (declare-sort U 0)
          (declare-fun f ( U ) U)
          ...
          (declare-fun x ( ) U)
          (assert (not (= (f (g x)) (f y))))
          ...
          (check-sat)
	  \end{verbatim}
  \end{enumerate}

\end{frame}
